bwd stuff

Rz/Algebra/PCA.lean
@@ -3,7 +3,7 @@ import Mathlib.Tactic.NthRewrite
 import Mathlib.Tactic.Use
 
 import Rz.Syntax.Magma
-import Rz.Data.Bwd
+-- import Rz.Data.Bwd
 
 universe u v w
 variable {α β : Type u}
@@ -19,7 +19,7 @@ class PAS (α : Type u) where
   ap_functional : {a₁ a₂ v₁ v₂ : α} → Ap a₁ a₂ v₁ → Ap a₁ a₂ v₂ → v₁ = v₂
 
 /-- Extend the small-step relation to a big-step relation on `FreeMagma α`. -/
-def PAS.Eval [PAS α] : (ρ : Bwd α) → FreeMagma α → α → Prop
+def PAS.Eval [PAS α] : (ρ : List α) → FreeMagma α → α → Prop
   | ρ, .var i, v => ∃ h, ρ.get ⟨i, h⟩ = v
   | _, .const a, v => a = v
   | ρ, .ap e₁ e₂, v => ∃ v₁ v₂, Eval ρ e₁ v₁ ∧ Eval ρ e₂ v₂ ∧ PAS.Ap v₁ v₂ v
@@ -30,11 +30,11 @@ macro_rules
 
 namespace PAS
 /-- `Undefined ρ e` denotes that an expression `e` diverges when evaluated in environment `ρ`. -/
-def Undefined [PAS α] (ρ : Bwd α) (e : FreeMagma α) : Prop := (a : α) → ¬ (ρ ⊢ e ⇓ a)
+def Undefined [PAS α] (ρ : List α) (e : FreeMagma α) : Prop := (a : α) → ¬ (ρ ⊢ e ⇓ a)
 /-- `Defined ρ e` denotes that an expression `e` diverges when evaluated in environment `ρ`. -/
-def Defined [PAS α] (ρ : Bwd α) (e : FreeMagma α) : Prop := ∃ (a : α), ρ ⊢ e ⇓ a
+def Defined [PAS α] (ρ : List α) (e : FreeMagma α) : Prop := ∃ (a : α), ρ ⊢ e ⇓ a
 /-- `Refines ρ e₁ e₂` denotes that an expression `e₂` is least as defined as `e₁`. -/
-def Refines [PAS α] (ρ₁ : Bwd α) (e₁ : FreeMagma α) (ρ₂ : Bwd α) (e₂ : FreeMagma α) : Prop := {a : α} → ρ₁ ⊢ e₁ ⇓ a → ρ₂ ⊢ e₂ ⇓ a
+def Refines [PAS α] (ρ₁ : List α) (e₁ : FreeMagma α) (ρ₂ : List α) (e₂ : FreeMagma α) : Prop := {a : α} → ρ₁ ⊢ e₁ ⇓ a → ρ₂ ⊢ e₂ ⇓ a
 end PAS
 
 @[inherit_doc PAS.Undefined]
@@ -57,7 +57,7 @@ namespace PAS
 -/
 
 /-- The refinement relation extends to a preorder on expressions. -/
-instance Refine [PAS α] {ρ : Bwd α} : Preorder (FreeMagma α) where
+instance Refine [PAS α] {ρ : List α} : Preorder (FreeMagma α) where
   le e₁ e₂ := PAS.Refines ρ e₁ ρ e₂
   le_refl e v v_eval := v_eval
   le_trans e₁ e₂ e₃ p q v v_eval := q (p v_eval)
@@ -65,7 +65,7 @@ variable [PAS α]
 
 /-- Application is monotonic with respect to refinement. -/
 theorem ap_le_ap
-  {ρ : Bwd α}
+  {ρ : List α}
   {e₁ e₂ e₁' e₂' : FreeMagma α}
   (le_left : ρ ⊢ e₁ ≤ ρ ⊢ e₁') (le_right : ρ ⊢ e₂ ≤ ρ ⊢ e₂')
   : ρ ⊢ e₁ e₂ ≤ ρ ⊢ e₁' e₂' := by
@@ -76,31 +76,31 @@ theorem ap_le_ap
 
 @[inherit_doc ap_le_ap]
 theorem ap_le_ap_right
-  {ρ : Bwd α}
+  {ρ : List α}
   {e₁ e₂ e₂' : FreeMagma α}
   (le_right : ρ ⊢ e₂ ≤ ρ ⊢ e₂')
   : ρ ⊢ e₁ e₂ ≤ ρ ⊢ e₁ e₂' := ap_le_ap (Refine.le_refl e₁) le_right
 
 @[inherit_doc ap_le_ap]
 theorem ap_le_ap_left
-  {ρ : Bwd α}
+  {ρ : List α}
   {e₁ e₂ e₁' : FreeMagma α}
   (le_left : ρ ⊢ e₁ ≤ ρ ⊢ e₁')
   : ρ ⊢ e₁ e₂ ≤ ρ ⊢ e₁' e₂ := ap_le_ap le_left (Refine.le_refl e₂)
 
 theorem ap_eval
-  {ρ : Bwd α}
+  {ρ : List α}
   {e₁ e₂ : FreeMagma α} {v : α}
   : ρ ⊢ e₁ e₂ ⇓ v ↔ ∃ v₁ v₂ : α, ρ ⊢ e₁ ⇓ v₁ ∧  ρ ⊢ e₂ ⇓ v₂ ∧ PAS.Ap v₁ v₂ v := by simp [PAS.Eval]
 
 theorem ap_congl
-  {ρ : Bwd α}
+  {ρ : List α}
   {e₁ e₂ : FreeMagma α} {v : α}
   : ρ ⊢ e₁ e₂ ⇓ v ↔ ∃ v₁ : α, ρ ⊢ e₁ ⇓ v₁ ∧ ρ ⊢ v₁ e₂ ⇓ v := by
   simp [PAS.Eval]
 
 theorem ap_congr
-  {ρ : Bwd α}
+  {ρ : List α}
   {e₁ e₂ : FreeMagma α} {v : α}
   : ρ ⊢ e₁ e₂ ⇓ v ↔ ∃ v₂ : α, ρ ⊢ e₂ ⇓ v₂ ∧ ρ ⊢ e₁ v₂ ⇓ v := by
   simp [PAS.Eval]
@@ -111,7 +111,7 @@ theorem ap_congr
     exact ⟨ v₁ , v₁_eval , v₂ , v₂_eval , v_ap ⟩
 
 @[simp] theorem const_eval
-  {ρ : Bwd α}
+  {ρ : List α}
   {a v : α}
   : ρ ⊢ a ⇓ v ↔ a = v := by
   simp [PAS.Eval]
@@ -122,7 +122,7 @@ theorem ap_congr
 
 /-- Evaluation is a functional relation. -/
 theorem eval_functional
-    {ρ : Bwd α}
+    {ρ : List α}
     {e : FreeMagma α} {a a' : α}
     (h1 : ρ ⊢ e ⇓ a) (h2 : ρ ⊢ e ⇓ a')
     : a = a' := by
@@ -148,9 +148,9 @@ class PCA (α : Type u) extends PAS α where
   /-- PCAs are equipped with a bracket abstraction operator. -/
   abs : FreeMagma α → FreeMagma α
   /-- Bracket abstraction yields a value. -/
-  abs_defined : (ρ : Bwd α) → (e : FreeMagma α) → ρ ⊢ $(abs e) ↓
+  abs_defined : (ρ : List α) → (e : FreeMagma α) → ρ ⊢ $(abs e) ↓
   /-- Bracket abstraction has a β-law. -/
-  abs_eval : {ρ : Bwd α} → {e₁ e₂ : FreeMagma α} → {v₁ : α} → ρ ⊢ $(abs e₁) e₂ ⇓ v₁ ↔ (∃ v₂, ρ ⊢ e₂ ⇓ v₂ ∧ (ρ :# v₂) ⊢ e₁ ⇓ v₁)
+  abs_eval : {ρ : List α} → {e₁ e₂ : FreeMagma α} → {v₁ : α} → ρ ⊢ $(abs e₁) e₂ ⇓ v₁ ↔ (∃ v₂, ρ ⊢ e₂ ⇓ v₂ ∧ (v₂ :: ρ) ⊢ e₁ ⇓ v₁)
 
 namespace PCA
 
@@ -162,47 +162,63 @@ def absn (e : FreeMagma α) (n : Nat) : FreeMagma α :=
   | n+1 => (absn (abs e) n)
 
 theorem absn_le
-  {ρ : Bwd α} {e : FreeMagma α} {as : Bwd (FreeMagma α)} {v : α} {vargs : Bwd α}
+  {ρ : List α} {e : FreeMagma α} {as : List (FreeMagma α)} {v : α} {vargs : List α}
   (e_eval : ρ ⊢ $(absn e as.length) $[as]* ⇓ v)
-  (h : as.length = vargs.length)
-  (as_eval : ∀ (i : Fin as.length), ρ ⊢ $(as.get i) ⇓ vargs.get (Fin.cast h i))
-  : (ρ ++ vargs) ⊢ e ⇓ v := by
-    match as, vargs with
-    | .nil, .nil =>
+  (as_eval : as.Forall₂ (fun a v => ρ ⊢ a ⇓ v) vargs)
+  : (vargs ++ ρ) ⊢ e ⇓ v := by
+    induction as_eval generalizing e v with
+    | nil =>
       simp [absn] at *
       exact e_eval
-    | .snoc as a, .snoc vargs varg =>
-      simp [absn, Bwd.foldBwd_snoc] at *
+    | @cons a varg as vargs a_eval _ IH =>
+      simp [absn] at *
       have ⟨ vbody , vbody_eval , v_ap ⟩ := PAS.ap_congl.1 e_eval
-      have ih_eval := absn_le (vargs := vargs) vbody_eval sorry sorry
-      have a_eval := as_eval 0
-      simp at a_eval
-      have outer_eval : (ρ ++ vargs) ⊢ $(abs e) varg ⇓ v := by
+      have' ih_eval := IH vbody_eval
+      have outer_eval : (vargs ++ ρ) ⊢ $(abs e) varg ⇓ v := by
         rw [PAS.ap_congl]
-        use _, ih_eval
-        sorry
-        -- simp [PAS.Eval]
-        -- sorry
-      have ⟨ varg', varg_eq, final_eval ⟩ := abs_eval.1 outer_eval
-      simp at varg_eq
-      rwa [varg_eq]
+        use vbody, ih_eval
+        have ⟨v', h1, h2⟩ := PAS.ap_congr.1 v_ap
+        rwa [← PAS.eval_functional a_eval h1] at h2
+      simpa [abs_eval] using outer_eval
+
+-- theorem le_absn
+--     {ρ : List α} {e : FreeMagma α} {as : List (FreeMagma α)} {v : α}
+--     : ρ ⊢ $(absn e as.length) $[as]* ⇓ v ↔
+--       ∃ vargs, as.Forall₂ (fun a v => ρ ⊢ a ⇓ v) vargs ∧ (vargs ++ ρ) ⊢ e ⇓ v := by
+--   constructor
+--   · intro e_eval
+--     induction as generalizing e v with
+--     | nil =>
+--       simp [absn] at *
+--       exact ⟨[], .nil, e_eval⟩
+--     | cons a as IH =>
+--       simp [absn] at *
+--       have ⟨ vbody , vbody_eval , v_ap ⟩ := PAS.ap_congl.1 e_eval
+--       have' ih_eval := IH vbody_eval
+--       have outer_eval : (vargs ++ ρ) ⊢ $(abs e) varg ⇓ v := by
+--         rw [PAS.ap_congl]
+--         use vbody, ih_eval
+--         have ⟨v', h1, h2⟩ := PAS.ap_congr.1 v_ap
+--         rwa [← PAS.eval_functional a_eval h1] at h2
+--       simpa [abs_eval] using outer_eval
+--   · done
 
 protected def id : FreeMagma α :=
   abs (.var 0)
 
-protected theorem id_le (ρ : Bwd α) (e : FreeMagma α) : ρ ⊢ PCA.id e ≤ ρ ⊢ e := by
+protected theorem id_le (ρ : List α) (e : FreeMagma α) : ρ ⊢ PCA.id e ≤ ρ ⊢ e := by
   intro v v_eval
   rewrite [PCA.id, PCA.abs_eval] at v_eval
   simp [PAS.Eval] at v_eval
   exact v_eval
 
-protected theorem le_id (ρ : Bwd α) (e : FreeMagma α) : ρ ⊢ e ≤ ρ ⊢ PCA.id e := by
+protected theorem le_id (ρ : List α) (e : FreeMagma α) : ρ ⊢ e ≤ ρ ⊢ PCA.id e := by
   intro v v_eval
   simp [PCA.id, PCA.abs_eval]
   simp [PAS.Eval]
   exact v_eval
 
-@[simp] protected theorem i_eval {ρ : Bwd α} {e : FreeMagma α} {v : α} : ρ ⊢ PCA.id e ⇓ v ↔ ρ ⊢ e ⇓ v :=
+@[simp] protected theorem i_eval {ρ : List α} {e : FreeMagma α} {v : α} : ρ ⊢ PCA.id e ⇓ v ↔ ρ ⊢ e ⇓ v :=
   ⟨ PCA.id_le _ _ , PCA.le_id _ _ ⟩
 
 -- \f g x.
@@ -210,22 +226,22 @@ protected def comp : FreeMagma α :=
   abs (abs (abs («magma» `(1) (`(2) `(0)))))
 
 protected theorem comp_le
-  {ρ : Bwd α} {e₁ e₂ e₃ : FreeMagma α} {v : α}
+  {ρ : List α} {e₁ e₂ e₃ : FreeMagma α} {v : α}
   : ρ ⊢ PCA.comp e₁ e₂ e₃ ≤ ρ ⊢ e₂ (e₁ e₃) := by
   intro v v_eval
   sorry
 
 protected theorem le_comp
-  {ρ : Bwd α} {e₁ e₂ e₃ : FreeMagma α} {v : α}
+  {ρ : List α} {e₁ e₂ e₃ : FreeMagma α} {v : α}
   : ρ ⊢ e₂ (e₁ e₃) ≤ ρ ⊢ PCA.comp e₁ e₂ e₃ :=
   sorry
 
 
 @[simp] protected theorem comp_eval
-  {ρ : Bwd α} {e₁ e₂ e₃ : FreeMagma α} {v : α}
+  {ρ : List α} {e₁ e₂ e₃ : FreeMagma α} {v : α}
   : ρ ⊢ PCA.comp e₁ e₂ e₃ ⇓ v ↔ ρ ⊢ e₂ (e₁ e₃) ⇓ v :=
   ⟨ PCA.comp_le (v := v) , PCA.le_comp (v := v) ⟩
--- @[simp] protected def comp_eval {ρ : Bwd α} {e₁ e₂ e₃ : FreeMagma α} {v : α} : ρ ⊢ PCA.comp e ⇓ v ↔ ρ ⊢ e ⇓ v := sorry
+-- @[simp] protected def comp_eval {ρ : List α} {e₁ e₂ e₃ : FreeMagma α} {v : α} : ρ ⊢ PCA.comp e ⇓ v ↔ ρ ⊢ e ⇓ v := sorry
 
 -- protected def le_comp (ρ : Bwd α) (e₁ e₂ e₃ : FreeMagma α) : ρ ⊢ e₂ (e₁ e₃) ≤ ρ ⊢ PCA.comp e₁ e₂ e₃ := by
 --   apply PAS.ap_le_ap_var_right
